Complete LinkedList module with references and stuff. Only the pop option is implemented, manual memory management is still TODO

test/LinkedList.fst
@@ -3,107 +3,188 @@ module LinkedList
 module B = FStar.Buffer
 module HS = FStar.HyperStack
 module G = FStar.Ghost
+module L = FStar.List.Tot
 
 open FStar.HyperStack.ST
 
 /// We revisit the classic example of lists, but in a low-level setting, using
 /// linked lists. This first version uses `ref`, the type of references that are
-/// always live.
+/// always live. However, we don't cheat and recall liveness "for free".
 noeq
-type linked_cell (a: Type0) =
-  | Nil: linked_cell a
+type t (a: Type0) =
+  ref (cell a)
+
+and cell (a: Type0) =
+  | Nil: cell a
   | Cons:
-      next: ref (linked_cell a) ->
+      next: t a ->
       data: a ->
-      linked_cell a
+      cell a
 
 /// Since linked lists go through a reference for indirection purposes, we
 /// enrich lists with a predicate that captures their length.
-let rec cell_has_length #a (h: HS.mem) (c: linked_cell a) (l: nat): GTot bool (decreases l) =
-  match c with
+let rec list_has_length #a (h: HS.mem) (c: t a) (l: nat):
+  GTot bool (decreases l)
+=
+  match HS.sel h c with
   | Nil -> l = 0
   | Cons next _ ->
       if l = 0 then
         false
       else
-        cell_has_length h (HS.sel h next) (l - 1)
+        list_has_length h next (l - 1)
+
+/// Note: a tempting solution might be to enrich the type of cells with an
+/// erased length that contains the "built-in" existentially quantified,
+/// proof-only, computationally-irrelevant length. This would, in turn,
+/// guarantee erasure by KreMLin and we would recover the type of linked lists
+/// that we hope for. This is tedious in practice, as the normalizer does not
+/// reduce underneath an `erased t`, leading to considerable type-checking
+/// difficulties.
 
 /// This lemma ensures that when matching on a Cons cell, then recursively
 /// calling something on length (l - 1), we get automatically that (l - 1) is
 /// nat.
-let cons_nonzero_length #a (h: HS.mem) (c: linked_cell a) (l: nat):
+let cons_nonzero_length #a (h: HS.mem) (c: ref (cell a)) (l: nat):
   Lemma
-    (requires (cell_has_length h c l /\ Cons? c))
+    (requires (list_has_length h c l /\ Cons? (HS.sel h c)))
     (ensures (l <> 0))
-    [ SMTPat (cell_has_length h c l); SMTPat (Cons? c) ] =
+    [ SMTPat (list_has_length h c l); SMTPat (Cons? (HS.sel h c)) ] =
     ()
 
-let rec length_unique #a (h: HS.mem) (c: linked_cell a) (l1 l2: nat):
+let rec length_injective #a (h: HS.mem) (c: ref (cell a)) (l1 l2: nat):
   Lemma
-    (requires (cell_has_length h c l1 /\ cell_has_length h c l2))
+    (requires (list_has_length h c l1 /\ list_has_length h c l2))
     (ensures (l1 = l2))
     (decreases l1)
-    [ SMTPat (cell_has_length h c l1); SMTPat (cell_has_length h c l2) ] =
-  match c with
+    [ SMTPat (list_has_length h c l1); SMTPat (list_has_length h c l2) ] =
+  match HS.sel h c with
   | Nil -> ()
   | Cons next _ ->
       // Without `cons_nonzero_length`, we would need assert (l1 <> 0)
-      length_unique h (HS.sel h next) (l1 - 1) (l2 - 1)
+      length_injective h next (l1 - 1) (l2 - 1)
 
-/// We pass lists by reference; so, a linked list is just a reference to a cell.
-type linked_list (a: Type0) =
-  ref (linked_cell a)
-
-/// This predicate states that are the cells are live. It relies on
-/// `cell_has_length` for its termination.
+/// A predicate that states that a single reference (the cell) is live.
 /// TODO: figure out why the predicate is called contains instead of live
-let rec cell_is_live #a #n (h: HS.mem) (c: linked_cell a {cell_has_length h c n})
-: Tot Type (decreases n)
+/// TODO: figure out why we need frameOf (see note to Aseem)
+let cell_is_live #a (h: HS.mem) (c: t a) =
+  HS.frameOf c = HS.root /\
+  HS.contains h c
+
+/// This predicate states that all the cells are live. It relies on
+/// `list_has_length` for its termination.
+/// TODO: figure out why `cell_is_live h l /\ (match ...)` doesn't work.
+let rec list_is_live #a #n (h: HS.mem) (l: t a {list_has_length h l n}):
+  Tot Type (decreases n)
 =
-  match c with
+  match HS.sel h l with
   | Nil ->
+      cell_is_live h l /\
       True
   | Cons next _ ->
-      HS.frameOf next = HS.root /\
-      HS.contains h next /\
-      cell_is_live #a #(n - 1) h (HS.sel h next)
+      cell_is_live h l /\
+      list_is_live #a #(n - 1) h next
 
-/// A live list is a live reference, that points to a live series of cells. We
-/// state that there exists an (unknown) length for this list.
-let list_is_live #a (h: HS.mem) (l: linked_list a) =
-  HS.frameOf l = HS.root /\ HS.contains h l /\ (
-  let c = HS.sel h l in
-  exists n. cell_has_length h c n /\ cell_is_live #a #n h c)
+/// This form will rarely turn out to be useful, except perhaps for user code.
+/// Indeed, we most often want to tie the length of the list in the final state
+/// with its length in the original state.
+let live #a (h: HS.mem) (l: t a) =
+  exists n. list_has_length h l n /\ list_is_live #a #n h l
 
-let list_next_live #a (h: HS.mem) (l: linked_list a):
+
+/// As we start proving some degree of functional correctness, we will have to
+/// reason about non-interference, and state that some operations do not modify
+/// the footprint of a given list.
+/// TODO: proper patterns for quantifiers!
+#set-options "--max_ifuel 0 --max_fuel 1"
+val footprint: (#a: Type) -> (#n: nat) -> (h: HS.mem) -> (l: t a) -> Ghost (list (ref (cell a)))
+  (requires (
+    list_has_length h l n /\
+    list_is_live #a #n h l
+  ))
+  (ensures (fun refs ->
+    let n_refs = L.length refs in
+    n_refs = n /\
+    (forall (i: nat). i < n ==>
+      list_has_length h (L.index refs (n - 1 - i)) (i + 1) /\
+      cell_is_live #a h (L.index refs (n - 1 - i)))
+  ))
+
+let rec footprint #a #n h l =
+  match HS.sel h l with
+  | Nil ->
+      []
+  | Cons next _ ->
+      let refs = footprint #a #(n - 1) h next in
+      l :: refs
+#reset-options
+
+/// An intermediary lemma, for sanity (it is currently unused): the head is
+/// disjoint from anything found in the footprint of the tail. The
+/// list_has_length predicate provides an easy contradiction if it were the
+/// case.
+/// TODO: pattern!
+let list_next_disjoint_i (#a: Type) (#n: nat) (h: HS.mem) (l: t a) (i: nat):
   Lemma
-    (requires (list_is_live h l /\ Cons? (HS.sel h l)))
-    (ensures (list_is_live h (Cons?.next (HS.sel h l))))
+    (requires (
+      list_has_length h l n /\
+      list_is_live #a #n h l /\
+      i < n - 1 /\
+      Cons? (HS.sel h l)))
+    (ensures (
+      let next = Cons?.next (HS.sel h l) in
+      let refs = footprint #a #(n - 1) h next in
+      HS.as_addr l <> HS.as_addr (L.index refs i)
+    ))
 =
   ()
 
-let list_next_disjoint #a (h: HS.mem) (l: linked_list a):
+/// All the reasoning about the pop operation is done in this lemma. If `head`
+/// is not found in the footprint of `l`, then the specific write we perform for
+/// pop (we could be more generic!) leaves the two essential predicates
+/// untouched for l.
+val pop_preserves_live: (#a: Type) -> (#n: nat) -> (h0: HS.mem) -> (head: ref (cell a)) -> (l: t a) ->
   Lemma
-    (requires (list_is_live h l /\ Cons? (HS.sel h l)))
-    (ensures (HS.as_addr l <> HS.as_addr (Cons?.next (HS.sel h l))))
-=
-  ()
+    (requires (
+      live h0 head /\
+      Cons? (HS.sel h0 head) /\
+      list_has_length h0 l n /\
+      list_is_live #a #n h0 l /\ (
+      let refs = footprint #a #n h0 l in
+      forall (i: nat). i < n ==> HS.as_addr head <> HS.as_addr (L.index refs i)
+    )))
+    (ensures (
+      live h0 head /\
+      Cons? (HS.sel h0 head) /\ (
+      let next = Cons?.next (HS.sel h0 head) in
+      let h1 = HS.upd h0 head (HS.sel h0 next) in
+      list_has_length h1 l n /\
+      list_is_live #a #n h1 l
+    )))
+    (decreases n)
+    [ SMTPat (list_is_live #a #n h0 l); SMTPat (Cons? (HS.sel h0 head)) ]
 
-val pop: (#a: Type) -> (l: linked_list a) ->
+#set-options "--z3rlimit 40 --max_ifuel 0"
+let rec pop_preserves_live #a #n h0 head l =
+  match HS.sel h0 l with
+  | Nil -> ()
+  | Cons l' _ ->
+      pop_preserves_live #a #(n - 1) h0 head l'
+
+val pop: (#a: Type) -> (#n: nat) -> (l: t a) ->
   ST (option a)
-  (requires (fun h -> list_is_live h l))
-  (ensures (fun h0 _ h1 -> True))//list_is_live h1 l))
-let pop #a l =
+  (requires (fun h -> list_has_length h l n /\ list_is_live #a #n h l))
+  (ensures (fun h0 v h1 ->
+    match v with
+    | None -> list_has_length h1 l n /\ list_is_live #a #n h1 l
+    | Some _ -> n > 0 /\ list_has_length h1 l (n - 1) /\ list_is_live #a #(n - 1) h1 l
+  ))
+
+let pop #a #n l =
   match !l with
   | Nil -> None
   | Cons next data ->
       let h0 = get () in
-      list_next_disjoint h0 l;
-      list_next_live h0 l;
-      assert (list_is_live h0 l);
-      assert (list_is_live h0 next);
       l := !next;
-      let h1 = get () in
-      assert (HS.sel h0 next == HS.sel h1 next);
-      assert (list_is_live h1 next);
+      pop_preserves_live #a #(n - 1) h0 l next;
       Some data
